# baseURI: http://www.inf.bi.ruhr-uni-bochum.de/loinontology
# prefix: loin

@prefix loin: <http://www.inf.bi.ruhr-uni-bochum.de/loinontology#> .
@prefix dc: <http://purl.org/dc/terms/> .
@prefix Container: <https://standards.iso.org/iso/21597/-1/ed-1/en/Container#> .
@prefix Linkset: <https://standards.iso.org/iso/21597/-1/ed-1/en/Linkset#> .
@prefix foaf: <http://xmlns.com/foaf/0.1#> .
@prefix vann: <http://purl.org/vocab/vann/> .
@prefix owl: <http://www.w3.org/2002/07/owl#> .
@prefix rdf: <http://www.w3.org/1999/02/22-rdf-syntax-ns#> .
@prefix rdfs: <http://www.w3.org/2000/01/rdf-schema#> .
@prefix sh: <http://www.w3.org/ns/shacl#> .
@prefix xsd: <http://www.w3.org/2001/XMLSchema#> .

<http://www.inf.bi.ruhr-uni-bochum.de/loinontology>
  rdf:type owl:Ontology ;
  dc:created "2023-01-30"^^xsd:date ;
  dc:creator [
      rdf:type foaf:Person ;
      foaf:name "Liu Liu, Ruhr University Bochum" ;
    ] ;
  dc:creator [
      rdf:type foaf:Person ;
      foaf:name "Philipp Hagedorn, Ruhr University Bochum" ;
    ] ;
  dc:description "The Level of Information Need (LOIN) Ontology is defined for specifying the information requirements. The LOIN ontology is based on BS EN 17412-1 (2020). Furthermore, it is specified with IDS developed by buildingSMART International and Information container for linked document delivery (ICDD) ISO 21597-1 (2020), "@en ;
  dc:publisher [
      rdf:type foaf:Organization ;
      foaf:name "Chair of Computing in Engineering, Ruhr University Bochum" ;
    ] ;
  dc:rights "Copyright 2023 by Chair of Computing in Engineering, Ruhr University Bochum" ;
  dc:source "https://github.com/RUB-Informatik-im-Bauwesen/loin"^^xsd:anyURI ;
  dc:title "Level of Information Need Ontology (LOIN)"@en ;
  vann:preferredNamespacePrefix "loin" ;
  owl:imports <https://standards.iso.org/iso/21597/-1/ed-1/en/Container> ;
  owl:imports <https://standards.iso.org/iso/21597/-1/ed-1/en/Linkset> ;
  owl:versionInfo "0.1" ;
.
loin:Actor
  rdf:type owl:Class ;
  rdfs:comment "Actor is a contextual aspect according to BS EN 17412-1 (2020)" ;
  rdfs:label "Actor" ;
  rdfs:subClassOf rdfs:Resource ;
.
loin:Appearance
  rdf:type owl:Class ;
  rdfs:comment "Appearance as a geometrical information specification for information need according to BS EN 17412-1 (2020)" ;
  rdfs:label "Appearance" ;
  rdfs:subClassOf loin:GeometrySpecification ;
.
loin:Attribute
  rdf:type owl:Class ;
  rdfs:comment "Attribut is an IDS facet according to IDS developed by buildingSMART International" ;
  rdfs:label "Attribut" ;
  rdfs:subClassOf loin:IDSFacetDefinition ;
  rdfs:subClassOf [
      rdf:type owl:Restriction ;
      owl:cardinality "1"^^xsd:nonNegativeInteger ;
      owl:onProperty loin:hasAttributeName ;
    ] ;
.
loin:AttributeName
  rdf:type owl:Class ;
  rdfs:comment "Attribute name must be a valid attribute name from the IFC schema according to IDS developed by buildingSMART International. Example AttributeName = \"Description\"" ;
  rdfs:label "Attribute name" ;
  rdfs:subClassOf loin:IDSFacetParameter ;
  rdfs:subClassOf [
      rdf:type owl:Restriction ;
      owl:cardinality "1"^^xsd:nonNegativeInteger ;
      owl:onProperty loin:RestrictionFormulation ;
    ] ;
  rdfs:subClassOf [
      rdf:type owl:Restriction ;
      owl:hasValue loin:SimpleValue ;
      owl:onProperty loin:hasRestrictionType ;
    ] ;
.
loin:Bounds
  rdf:type loin:IDSRestrictionType ;
.
loin:BreakdownStructure
  rdf:type owl:Class ;
  rdfs:comment "Breakdown structure is a term for positioning the object in a structure according to BS EN 17412-1 (2020)" ;
  rdfs:label "Breakdown structure" ;
  rdfs:subClassOf rdfs:Resource ;
  rdfs:subClassOf [
      rdf:type owl:Restriction ;
      owl:cardinality "1"^^xsd:nonNegativeInteger ;
      owl:onProperty loin:hasIdentifier ;
    ] ;
.
loin:BreakdownStructureType
  rdf:type owl:Class ;
  rdfs:comment "Breakdown structure type is a term to specify the structure according to BS EN 17412-1 (2020)" ;
  rdfs:label "Breakdown structure type" ;
  rdfs:subClassOf rdfs:Resource ;
.
loin:Classification
  rdf:type owl:Class ;
  rdfs:comment "Classification is an IDS facet according to IDS developed by buildingSMART International" ;
  rdfs:label "Classification" ;
  rdfs:subClassOf loin:IDSFacetDefinition ;
  owl:equivalentClass loin:Identification ;
.
loin:ClassificationSystem
  rdf:type loin:BreakdownStructureType ;
  rdfs:comment "An example of breakdown structure type according to BS EN 17412-1 (2020)" ;
  rdfs:label "Classification system" ;
.
loin:Codification
  rdf:type loin:IdentifierType ;
  rdfs:label "Codification of an item in a breakdown structure" ;
.
loin:Description
  rdf:type owl:AnnotationProperty ;
  rdfs:range xsd:string ;
.
loin:Detail
  rdf:type owl:Class ;
  rdfs:comment "Detail as a geometrical information specification for information need according to BS EN 17412-1 (2020)" ;
  rdfs:label "Detail" ;
  rdfs:subClassOf loin:GeometrySpecification ;
.
loin:Dimensionality
  rdf:type owl:Class ;
  rdfs:comment "Dimensionality as a geometrical information specification for information need according to BS EN 17412-1 (2020)" ;
  rdfs:label "Dimensionality" ;
  rdfs:subClassOf loin:GeometrySpecification ;
.
loin:Document
  rdf:type owl:Class ;
  rdfs:comment "Document is a term for specifying the documentation of information need according to BS EN 17412-1 (2020)" ;
  rdfs:label "Document" ;
  rdfs:subClassOf rdfs:Resource ;
  rdfs:subClassOf [
      rdf:type owl:Restriction ;
      owl:maxCardinality "1"^^xsd:nonNegativeInteger ;
      owl:onProperty loin:belongsToInformationContent ;
    ] ;
  rdfs:subClassOf [
      rdf:type owl:Restriction ;
      owl:maxCardinality "1"^^xsd:nonNegativeInteger ;
      owl:onProperty loin:isRelatedToContainerDocument ;
    ] ;
  rdfs:subClassOf [
      rdf:type owl:Restriction ;
      owl:maxCardinality "1"^^xsd:nonNegativeInteger ;
      owl:onProperty loin:isRelatedToContainerLinkset ;
    ] ;
  rdfs:subClassOf [
      rdf:type owl:Restriction ;
      owl:onProperty loin:hasDocumentSpecification ;
      owl:someValuesFrom loin:DocumentContent ;
    ] ;
  rdfs:subClassOf [
      rdf:type owl:Restriction ;
      owl:onProperty loin:hasDocumentSpecification ;
      owl:someValuesFrom loin:DocumentFormat ;
    ] ;
  rdfs:subClassOf [
      rdf:type owl:Restriction ;
      owl:onProperty loin:hasDocumentSpecification ;
      owl:someValuesFrom loin:DocumentPurpose ;
    ] ;
.
loin:DocumentContent
  rdf:type owl:Class ;
  rdfs:comment "Document specification for content for information need according to BS EN 17412-1 (2020)" ;
  rdfs:label "Document content" ;
  rdfs:subClassOf loin:DocumentSpecification ;
.
loin:DocumentFormat
  rdf:type owl:Class ;
  rdfs:comment "Document specification for format for information need according to BS EN 17412-1 (2020)" ;
  rdfs:label "Document format" ;
  rdfs:subClassOf loin:DocumentSpecification ;
.
loin:DocumentPurpose
  rdf:type owl:Class ;
  rdfs:comment "Document specification for purpose for information need according to BS EN 17412-1 (2020)" ;
  rdfs:label "Document purpose" ;
  rdfs:subClassOf loin:DocumentSpecification ;
.
loin:DocumentSpecification
  rdf:type owl:Class ;
  rdfs:comment "Additional specification of document for information need according to BS EN 17412-1 (2020)" ;
  rdfs:label "Document specification" ;
  rdfs:subClassOf rdfs:Resource ;
.
loin:Documentation
  rdf:type owl:Class ;
  rdfs:comment "Documentation is a term for specifying the information need according to BS EN 17412-1 (2020)" ;
  rdfs:label "Documentation" ;
  rdfs:subClassOf rdfs:Resource ;
.
loin:EngineeringPrinciple
  rdf:type loin:BreakdownStructureType ;
  rdfs:comment "An example of breakdown structure type according to BS EN 17412-1 (2020)" ;
  rdfs:label "Engineering principle" ;
.
loin:Entity
  rdf:type owl:Class ;
  rdfs:comment "Entity is an IDS facet according to IDS developed by buildingSMART International" ;
  rdfs:label "Entity" ;
  rdfs:subClassOf loin:IDSFacetDefinition ;
  rdfs:subClassOf [
      rdf:type owl:Restriction ;
      owl:cardinality "1"^^xsd:nonNegativeInteger ;
      owl:onProperty loin:hasEntityName ;
    ] ;
.
loin:EntityName
  rdf:type owl:Class ;
  rdfs:comment "Entity name must be a valid IFC class from the IFC schema according to IDS developed by buildingSMART International. Example EntityName = \"IFCWALL\"" ;
  rdfs:label "Entity name" ;
  rdfs:subClassOf loin:IDSFacetParameter ;
  rdfs:subClassOf [
      rdf:type owl:Restriction ;
      owl:cardinality "1"^^xsd:nonNegativeInteger ;
      owl:onProperty loin:hasRestrictionType ;
    ] ;
.
loin:Enumeration
  rdf:type loin:IDSRestrictionType ;
.
loin:FederationStrategy
  rdf:type loin:BreakdownStructureType ;
  rdfs:comment "An example of breakdown structure type according to BS EN 17412-1 (2020)" ;
  rdfs:label "Federation strategy" ;
.
loin:Functional
  rdf:type loin:BreakdownStructureType ;
  rdfs:comment "An example of breakdown structure type according to BS EN 17412-1 (2020)" ;
  rdfs:label "Functional structure" ;
.
loin:Geometry
  rdf:type owl:Class ;
  rdfs:comment "Geometrical information is a term for specifying the information need according to BS EN 17412-1 (2020)" ;
  rdfs:label "Geometrical information" ;
  rdfs:subClassOf rdfs:Resource ;
  rdfs:subClassOf [
      rdf:type owl:Restriction ;
      owl:cardinality "1"^^xsd:nonNegativeInteger ;
      owl:onProperty loin:requested ;
    ] ;
  rdfs:subClassOf [
      rdf:type owl:Restriction ;
      owl:onProperty loin:hasGeometrySpecification ;
      owl:someValuesFrom loin:Appearance ;
    ] ;
  rdfs:subClassOf [
      rdf:type owl:Restriction ;
      owl:onProperty loin:hasGeometrySpecification ;
      owl:someValuesFrom loin:Detail ;
    ] ;
  rdfs:subClassOf [
      rdf:type owl:Restriction ;
      owl:onProperty loin:hasGeometrySpecification ;
      owl:someValuesFrom loin:Dimensionality ;
    ] ;
  rdfs:subClassOf [
      rdf:type owl:Restriction ;
      owl:onProperty loin:hasGeometrySpecification ;
      owl:someValuesFrom loin:Location ;
    ] ;
  rdfs:subClassOf [
      rdf:type owl:Restriction ;
      owl:onProperty loin:hasGeometrySpecification ;
      owl:someValuesFrom loin:ParametricBehaviour ;
    ] ;
.
loin:GeometrySpecification
  rdf:type owl:Class ;
  rdfs:comment "Additional specification of geometrical information for information need according to BS EN 17412-1 (2020)" ;
  rdfs:label "Geometrical information specification" ;
  rdfs:subClassOf rdfs:Resource ;
.
loin:Handdrawn_Sketches
  rdf:type loin:DocumentContent ;
  rdfs:comment "Documents such as such as initial sketches, site plans" ;
.
loin:Hard_Copy
  rdf:type loin:DocumentContent ;
  rdfs:comment "Documents of geometrical information or alphanumerical information can also be considered as documents." ;
.
loin:IDSDataDefinition
  rdf:type owl:Class ;
  rdfs:comment "IDS data definition is used to specify the alphanumerical information according to IDS developed by buildingSMART International" ;
  rdfs:label "IDS data definition" ;
  rdfs:subClassOf loin:InformationContent ;
  rdfs:subClassOf [
      rdf:type owl:Restriction ;
      owl:cardinality "1"^^xsd:nonNegativeInteger ;
      owl:onProperty loin:description ;
    ] ;
  rdfs:subClassOf [
      rdf:type owl:Restriction ;
      owl:maxCardinality "0"^^xsd:nonNegativeInteger ;
      owl:onProperty loin:specifiedByIdentifier ;
    ] ;
  rdfs:subClassOf [
      rdf:type owl:Restriction ;
      owl:minCardinality "1"^^xsd:nonNegativeInteger ;
      owl:onProperty loin:hasApplicability ;
    ] ;
  rdfs:subClassOf [
      rdf:type owl:Restriction ;
      owl:minCardinality "1"^^xsd:nonNegativeInteger ;
      owl:onProperty loin:hasRequirement ;
    ] ;
  rdfs:subClassOf [
      rdf:type owl:Restriction ;
      owl:onProperty loin:hasApplicability ;
      owl:someValuesFrom loin:Entity ;
    ] ;
.
loin:IDSFacetDefinition
  rdf:type owl:Class ;
  rdf:type sh:NodeShape ;
  rdfs:comment "IDS facet definition is used to define a facet to apply the requirement or to require the information according to IDS developed by buildingSMART International" ;
  rdfs:label "IDS facet Definition" ;
  rdfs:subClassOf rdfs:Resource ;
.
loin:IDSFacetParameter
  rdf:type owl:Class ;
  rdfs:comment "IDS facet parameter is used to specify a facet definition according to IDS developed by buildingSMART International" ;
  rdfs:label "IDS facet parameter" ;
  rdfs:subClassOf rdfs:Resource ;
.
loin:IDSRequirementType
  rdf:type owl:Class ;
  rdfs:comment "IDS requirement type is used to specify a requirement, if it is optional or mandatory according to IDS developed by buildingSMART International" ;
  rdfs:label "IDS requirement type" ;
  rdfs:subClassOf rdfs:Resource ;
  owl:oneOf (
      "Required"
      "Optional"
      "Prohibited"
    ) ;
.
loin:IDSRestrictionType
  rdf:type owl:Class ;
  rdfs:comment "Restriction type is used to define the value of IDS facet parameter according to IDS developed by buildingSMART International" ;
  rdfs:label "Restriction type" ;
  rdfs:subClassOf rdfs:Resource ;
.
loin:IFCDataType
  rdf:type owl:Class ;
  rdfs:comment "IFC data type must be a valid predefined type from the IFC schema according to IDS developed by buildingSMART International" ;
  rdfs:label "IFC data type" ;
  rdfs:subClassOf loin:IDSFacetParameter ;
  rdfs:subClassOf [
      rdf:type owl:Restriction ;
      owl:cardinality "1"^^xsd:nonNegativeInteger ;
      owl:onProperty loin:RestrictionFormulation ;
    ] ;
  rdfs:subClassOf [
      rdf:type owl:Restriction ;
      owl:hasValue loin:SimpleValue ;
      owl:onProperty loin:hasRestrictionType ;
    ] ;
.
loin:Identification
  rdf:type owl:Class ;
  rdfs:comment "Identification is a term for positioning the object in a breakdown structure according to BS EN 17412-1 (2020)" ;
  rdfs:label "Identification" ;
  rdfs:subClassOf rdfs:Resource ;
  rdfs:subClassOf [
      rdf:type owl:Restriction ;
      owl:minCardinality "1"^^xsd:nonNegativeInteger ;
      owl:onProperty loin:hasBreakdownStructure ;
    ] ;
.
loin:Identifier
  rdf:type owl:Class ;
  rdfs:comment "Identifier is used to assiging a vaule for positioning the object in a breakdown structure according to BS EN 17412-1 (2020)" ;
  rdfs:label "Identifier" ;
  rdfs:subClassOf rdfs:Resource ;
  rdfs:subClassOf [
      rdf:type owl:Restriction ;
      owl:cardinality "1"^^xsd:nonNegativeInteger ;
      owl:onProperty loin:hasBreakdownStructure ;
    ] ;
  rdfs:subClassOf [
      rdf:type owl:Restriction ;
      owl:cardinality "1"^^xsd:nonNegativeInteger ;
      owl:onProperty loin:hasIdentifierType ;
    ] ;
  rdfs:subClassOf [
      rdf:type owl:Restriction ;
      owl:cardinality "1"^^xsd:nonNegativeInteger ;
      owl:onProperty loin:value ;
    ] ;
.
loin:IdentifierType
  rdf:type owl:Class ;
  rdfs:comment "Identifier type is used to specify the identifier in a breakdown structure according to BS EN 17412-1 (2020)" ;
  rdfs:label "Identifier type" ;
  rdfs:subClassOf rdfs:Resource ;
.
loin:Index
  rdf:type loin:IdentifierType ;
  rdfs:label "Index of an item in a breakdown structure" ;
.
loin:Information
  rdf:type owl:Class ;
  rdfs:comment "Alphanumerical information is a term for specifying the information need according to BS EN 17412-1 (2020)" ;
  rdfs:label "Alphanumerical information" ;
  rdfs:subClassOf rdfs:Resource ;
  rdfs:subClassOf [
      rdf:type owl:Restriction ;
      owl:cardinality "1"^^xsd:nonNegativeInteger ;
      owl:onProperty loin:requested ;
    ] ;
.
loin:InformationContent
  rdf:type owl:Class ;
  rdfs:comment "Alphanumerical information content is a term for specifying the alphanumerical information according to BS EN 17412-1 (2020)" ;
  rdfs:label "Alphanumerical information content" ;
  rdfs:subClassOf rdfs:Resource ;
.
loin:InformationDeliveryMilestone
  rdf:type owl:Class ;
  rdfs:comment "Information delivery milestone is a contextual aspect according to BS EN 17412-1 (2020)" ;
  rdfs:label "Information delivery milestone" ;
  rdfs:subClassOf rdfs:Resource ;
  rdfs:subClassOf [
      rdf:type owl:Restriction ;
      owl:cardinality "1"^^xsd:nonNegativeInteger ;
      owl:onProperty loin:hasProvider ;
    ] ;
  rdfs:subClassOf [
      rdf:type owl:Restriction ;
      owl:cardinality "1"^^xsd:nonNegativeInteger ;
      owl:onProperty loin:hasPurpose ;
    ] ;
  rdfs:subClassOf [
      rdf:type owl:Restriction ;
      owl:cardinality "1"^^xsd:nonNegativeInteger ;
      owl:onProperty loin:hasReceiver ;
    ] ;
  rdfs:subClassOf [
      rdf:type owl:Restriction ;
      owl:minCardinality "1"^^xsd:nonNegativeInteger ;
      owl:onProperty loin:hasObject ;
    ] ;
.
loin:InformationProvider
  rdf:type owl:Class ;
  rdfs:comment "Information provider is a party for information delivery according to ISO 19650-1 (2018)" ;
  rdfs:label "Information provider" ;
  rdfs:subClassOf loin:Actor ;
.
loin:InformationReceiver
  rdf:type owl:Class ;
  rdfs:comment "Information receiver is a party for information delivery according to ISO 19650-1 (2018)" ;
  rdfs:label "Information receiver" ;
  rdfs:subClassOf loin:Actor ;
.
loin:Length
  rdf:type loin:IDSRestrictionType ;
.
loin:Location
  rdf:type owl:Class ;
  rdfs:comment "Location as a geometrical information specification for information need according to BS EN 17412-1 (2020)" ;
  rdfs:label "Location" ;
  rdfs:subClassOf loin:GeometrySpecification ;
.
loin:Manual
  rdf:type loin:DocumentContent ;
  rdfs:comment "Documents such as maintenance and user manuals" ;
.
loin:Material
  rdf:type owl:Class ;
  rdfs:comment "Material is an IDS facet according to IDS developed by buildingSMART International" ;
  rdfs:label "Material" ;
  rdfs:subClassOf loin:IDSFacetDefinition ;
.
loin:Name
  rdf:type loin:IdentifierType ;
  rdfs:label "Name of an item in a breakdown structure" ;
.
loin:NotRequested
  rdf:type loin:Geometry ;
  loin:requested "false"^^xsd:boolean ;
.
loin:Numbering
  rdf:type loin:IdentifierType ;
  rdfs:label "Numbering of an item in a breakdown structure" ;
.
loin:Object
  rdf:type owl:Class ;
  rdfs:comment "Object is a contextual aspect according to BS EN 17412-1 (2020)" ;
  rdfs:label "Object" ;
  rdfs:subClassOf rdfs:Resource ;
  rdfs:subClassOf [
      rdf:type owl:Restriction ;
      owl:maxCardinality "1"^^xsd:nonNegativeInteger ;
      owl:onProperty loin:hasDocumentation ;
    ] ;
  rdfs:subClassOf [
      rdf:type owl:Restriction ;
      owl:maxCardinality "1"^^xsd:nonNegativeInteger ;
      owl:onProperty loin:hasGeometry ;
    ] ;
  rdfs:subClassOf [
      rdf:type owl:Restriction ;
      owl:maxCardinality "1"^^xsd:nonNegativeInteger ;
      owl:onProperty loin:hasInformation ;
    ] ;
.
loin:OntologyDataDefinition
  rdf:type owl:Class ;
  rdfs:comment "Ontology data definition is used to specify the alphanumerical information according to a published or customized ontology" ;
  rdfs:label "Ontology data definition" ;
  rdfs:subClassOf loin:InformationContent ;
  rdfs:subClassOf [
      rdf:type owl:Restriction ;
      owl:minCardinality "1"^^xsd:nonNegativeInteger ;
      owl:onProperty loin:specifiedByIdentifier ;
    ] ;
.
loin:ParametricBehaviour
  rdf:type owl:Class ;
  rdfs:comment "Parametric behaviour as a geometrical information specification for information need according to BS EN 17412-1 (2020)" ;
  rdfs:label "Parametric behaviour" ;
  rdfs:subClassOf loin:GeometrySpecification ;
.
loin:Pattern
  rdf:type loin:IDSRestrictionType ;
.
loin:Photograph
  rdf:type loin:DocumentContent ;
  rdfs:comment "Documents such as records of work done, records of existing conditions" ;
.
loin:PredefinedType
  rdf:type owl:Class ;
  rdfs:comment "Predefined type must be a valid predefined type from the IFC schema, or any custom text value according to IDS developed by buildingSMART International" ;
  rdfs:label "Predefined type" ;
  rdfs:subClassOf loin:IDSFacetParameter ;
  rdfs:subClassOf [
      rdf:type owl:Restriction ;
      owl:cardinality "1"^^xsd:nonNegativeInteger ;
      owl:onProperty loin:hasRestrictionType ;
    ] ;
.
loin:Property
  rdf:type owl:Class ;
  rdfs:comment "Property is an IDS facet according to IDS developed by buildingSMART International" ;
  rdfs:label "Property" ;
  rdfs:subClassOf loin:IDSFacetDefinition ;
  rdfs:subClassOf [
      rdf:type owl:Restriction ;
      owl:cardinality "1"^^xsd:nonNegativeInteger ;
      owl:onProperty loin:belongsToPset ;
    ] ;
  rdfs:subClassOf [
      rdf:type owl:Restriction ;
      owl:cardinality "1"^^xsd:nonNegativeInteger ;
      owl:onProperty loin:hasIFCDataType ;
    ] ;
  rdfs:subClassOf [
      rdf:type owl:Restriction ;
      owl:cardinality "1"^^xsd:nonNegativeInteger ;
      owl:onProperty loin:hasPropertyName ;
    ] ;
.
loin:PropertyName
  rdf:type owl:Class ;
  rdfs:comment "Property name must be a valid name from the IFC schema, or any custom text value according to IDS developed by buildingSMART International" ;
  rdfs:label "Property name" ;
  rdfs:subClassOf loin:IDSFacetParameter ;
  rdfs:subClassOf [
      rdf:type owl:Restriction ;
      owl:cardinality "1"^^xsd:nonNegativeInteger ;
      owl:onProperty loin:RestrictionFormulation ;
    ] ;
  rdfs:subClassOf [
      rdf:type owl:Restriction ;
      owl:hasValue loin:SimpleValue ;
      owl:onProperty loin:hasRestrictionType ;
    ] ;
.
loin:Provided_As_Information
  rdf:type loin:DocumentPurpose ;
  rdfs:label "The document delivered by Inquirer as percondition or information" ;
.
loin:PsetName
  rdf:type owl:Class ;
  rdfs:comment "Property set name must be a valid name from the IFC schema, or any custom text value according to IDS developed by buildingSMART International" ;
  rdfs:label "Property set name" ;
  rdfs:subClassOf loin:IDSFacetParameter ;
  rdfs:subClassOf [
      rdf:type owl:Restriction ;
      owl:cardinality "1"^^xsd:nonNegativeInteger ;
      owl:onProperty loin:RestrictionFormulation ;
    ] ;
  rdfs:subClassOf [
      rdf:type owl:Restriction ;
      owl:cardinality "1"^^xsd:nonNegativeInteger ;
      owl:onProperty loin:hasRestrictionType ;
    ] ;
.
loin:Purpose
  rdf:type owl:Class ;
  rdfs:comment "Purpose is a contextual aspect according to BS EN 17412-1 (2020)" ;
  rdfs:label "Purpose" ;
  rdfs:subClassOf rdfs:Resource ;
  rdfs:subClassOf [
      rdf:type owl:Restriction ;
      owl:cardinality "1"^^xsd:nonNegativeInteger ;
      owl:onProperty loin:description ;
    ] ;
.
loin:ReferenceOfStructure
  rdf:type loin:IdentifierType ;
  rdfs:label "Reference of an item in a breakdown structure" ;
.
loin:Report
  rdf:type loin:DocumentContent ;
.
loin:Required_For_Approval
  rdf:type loin:DocumentPurpose ;
  rdfs:label "The document required by deliverer for getting approval" ;
.
loin:Required_with_Supplement
  rdf:type loin:DocumentPurpose ;
  rdfs:label "The Document required by deliverer with supplement of information" ;
.
loin:RestrictionFormulation
  rdf:type owl:DatatypeProperty ;
  rdfs:domain loin:IDSFacetParameter ;
  rdfs:range xsd:string ;
.
loin:Semantic
  rdf:type loin:BreakdownStructureType ;
  rdfs:comment "An example of breakdown structure type according to BS EN 17412-1 (2020)" ;
  rdfs:label "Semantic structure" ;
.
loin:Signed_Document
  rdf:type loin:DocumentContent ;
  rdfs:comment "Documents such as such as test certificates, insurance policies, delivery notes" ;
.
loin:SimpleValue
  rdf:type loin:IDSRestrictionType ;
.
loin:Spatial
  rdf:type loin:BreakdownStructureType ;
  rdfs:comment "An example of breakdown structure type according to BS EN 17412-1 (2020)" ;
  rdfs:label "Spatial structure" ;
.
loin:Specification
  rdf:type loin:DocumentContent ;
.
loin:TypeName
  rdf:type loin:IdentifierType ;
  rdfs:label "Type name of an item in a breakdown structure" ;
.
loin:Used_As_Template
  rdf:type loin:DocumentPurpose ;
  rdfs:label "The document delivered by inquirer for using as template" ;
.
loin:Value
  rdf:type owl:Class ;
  rdfs:comment "Value can be any custom value according to IDS developed by buildingSMART International" ;
  rdfs:label "Value" ;
  rdfs:subClassOf loin:IDSFacetParameter ;
  rdfs:subClassOf [
      rdf:type owl:Restriction ;
      owl:cardinality "1"^^xsd:nonNegativeInteger ;
      owl:onProperty loin:RestrictionFormulation ;
    ] ;
  rdfs:subClassOf [
      rdf:type owl:Restriction ;
      owl:cardinality "1"^^xsd:nonNegativeInteger ;
      owl:onProperty loin:hasRestrictionType ;
    ] ;
.
loin:absolute
  rdf:type loin:Location ;
.
loin:belongsToInformationContent
  rdf:type owl:ObjectProperty ;
  rdfs:domain loin:Document ;
  rdfs:label "belongs to information content" ;
  rdfs:range loin:InformationContent ;
.
loin:belongsToPset
  rdf:type owl:ObjectProperty ;
  rdfs:domain loin:Property ;
  rdfs:label "belongs to Pset" ;
  rdfs:range loin:PsetName ;
.
loin:constructive
  rdf:type loin:ParametricBehaviour ;
.
loin:coordination
  rdf:type loin:Purpose ;
  loin:description "coordination - example from ISO 17412-1:2022 - Annex B" ;
  rdfs:comment "Example from ISO 17412-1:2022 - Annex B" ;
  rdfs:label "Coordination" ;
.
loin:costEstimation
  rdf:type loin:Purpose ;
  loin:description "Cost estimation - example from ISO 17412-1:2022 - Annex B" ;
  rdfs:comment "Example from ISO 17412-1:2022 - Annex B" ;
  rdfs:label "Cost estimation" ;
.
loin:description
  rdf:type owl:DatatypeProperty ;
  rdfs:domain [
      rdf:type owl:Class ;
      owl:unionOf (
          loin:InformationContent
          loin:Purpose
        ) ;
    ] ;
.
loin:detailed
  rdf:type loin:Detail ;
.
loin:detailedDesign
  rdf:type loin:InformationDeliveryMilestone ;
  rdfs:comment "Example from ISO 17412-1:2022 - Annex B" ;
  rdfs:label "Detailed design" ;
.
loin:explicit
  rdf:type loin:ParametricBehaviour ;
.
loin:finalDesign
  rdf:type loin:InformationDeliveryMilestone ;
  rdfs:comment "Example from ISO 17412-1:2022 - Annex B" ;
  rdfs:label "Final design" ;
.
loin:fireSmokeSimulation
  rdf:type loin:Purpose ;
  loin:description "Fire and smoke simulation - example from ISO 17412-1:2022 - Annex B" ;
  rdfs:comment "Example from ISO 17412-1:2022 - Annex B" ;
  rdfs:label "Fire and smoke simulation" ;
.
loin:hasAgent
  rdf:type owl:ObjectProperty ;
  rdfs:comment "Information of the information delivery actor defined by foaf ontology mit class foaf:Agent" ;
  rdfs:domain loin:Actor ;
  rdfs:label "has agent" ;
.
loin:hasAppearance
  rdf:type owl:ObjectProperty ;
  rdfs:label "has appearance" ;
  rdfs:range loin:Appearance ;
.
loin:hasApplicability
  rdf:type owl:ObjectProperty ;
  rdfs:comment "The object property describes the applicability of a facet for the specification" ;
  rdfs:domain loin:IDSDataDefinition ;
  rdfs:label "has applicability" ;
  rdfs:range loin:IDSFacetDefinition ;
.
loin:hasAttributeName
  rdf:type owl:ObjectProperty ;
  rdfs:domain loin:Attribute ;
  rdfs:label "has attribute name" ;
  rdfs:range loin:AttributeName ;
.
loin:hasBreakdownStructure
  rdf:type owl:ObjectProperty ;
  rdfs:domain loin:Identification ;
  rdfs:label "has breakdown structure" ;
  rdfs:range loin:BreakdownStructure ;
.
loin:hasBreakdownStructureType
  rdf:type owl:ObjectProperty ;
  rdfs:domain loin:BreakdownStructure ;
  rdfs:label "has breakdown structure type" ;
  rdfs:range loin:BreakdownStructureType ;
.
loin:hasDetail
  rdf:type owl:ObjectProperty ;
  rdfs:label "has detail" ;
  rdfs:range loin:Detail ;
.
loin:hasDimensionality
  rdf:type owl:ObjectProperty ;
  rdfs:label "has dimensionality" ;
  rdfs:range loin:Dimensionality ;
.
loin:hasDocument
  rdf:type owl:ObjectProperty ;
  rdfs:domain loin:Documentation ;
  rdfs:label "has document" ;
.
loin:hasDocumentSpecification
  rdf:type owl:ObjectProperty ;
  rdfs:domain loin:Document ;
  rdfs:label "has documentaton specification" ;
  rdfs:range loin:DocumentSpecification ;
.
loin:hasDocumentation
  rdf:type owl:ObjectProperty ;
  rdfs:domain loin:Object ;
  rdfs:label "has documentation" ;
  rdfs:range loin:Documentation ;
.
loin:hasEntityName
  rdf:type owl:ObjectProperty ;
  rdfs:domain loin:Entity ;
  rdfs:label "has entity name" ;
  rdfs:range loin:EntityName ;
.
loin:hasGeometry
  rdf:type owl:ObjectProperty ;
  rdfs:domain loin:Object ;
  rdfs:label "has geometrical information" ;
  rdfs:range loin:Geometry ;
.
loin:hasGeometrySpecification
  rdf:type owl:ObjectProperty ;
  rdfs:comment """[\"Appearance\",
\"Detail\",
\"Dimensionality\",
\"Location\",
\"ParametricBehaviour\"]""" ;
  rdfs:domain loin:Geometry ;
  rdfs:label "has geometrical information specification" ;
  rdfs:range loin:GeometrySpecification ;
.
loin:hasIFCDataType
  rdf:type owl:ObjectProperty ;
  rdfs:domain loin:Property ;
  rdfs:label "has IFC data type" ;
  rdfs:range loin:IFCDataType ;
.
loin:hasIdentification
  rdf:type owl:ObjectProperty ;
  rdfs:domain loin:Information ;
  rdfs:label "has identification" ;
  rdfs:label "hasTypeOfBreakdownStructure" ;
  rdfs:range loin:Identification ;
.
loin:hasIdentifier
  rdf:type owl:ObjectProperty ;
  rdfs:domain loin:BreakdownStructure ;
  rdfs:label "has identifier" ;
  rdfs:range loin:Identifier ;
.
loin:hasIdentifierType
  rdf:type owl:ObjectProperty ;
  rdfs:domain loin:Identifier ;
  rdfs:label "has identifier type" ;
  rdfs:range loin:IdentifierType ;
.
loin:hasInformation
  rdf:type owl:ObjectProperty ;
  rdfs:domain loin:Object ;
  rdfs:label "has alphanumerical information" ;
  rdfs:range loin:Information ;
.
loin:hasInformationContent
  rdf:type owl:ObjectProperty ;
  rdfs:domain loin:Information ;
  rdfs:label "has alphanumerical informaton content" ;
  rdfs:range loin:InformationContent ;
.
loin:hasLocation
  rdf:type owl:ObjectProperty ;
  rdfs:label "has location" ;
  rdfs:range loin:Location ;
.
loin:hasObject
  rdf:type owl:ObjectProperty ;
  rdfs:domain loin:InformationDeliveryMilestone ;
  rdfs:label "has object" ;
  rdfs:range loin:Object ;
.
loin:hasParameterValue
  rdf:type owl:ObjectProperty ;
  rdfs:label "has parameter value" ;
.
loin:hasParametricBehaviour
  rdf:type owl:ObjectProperty ;
  rdfs:label "has parametric behaviour" ;
  rdfs:range loin:ParametricBehaviour ;
.
loin:hasPredefinedType
  rdf:type owl:ObjectProperty ;
  rdfs:domain loin:Entity ;
  rdfs:label "has predefined type" ;
  rdfs:range loin:PredefinedType ;
.
loin:hasPropertyName
  rdf:type owl:ObjectProperty ;
  rdfs:domain loin:Property ;
  rdfs:label "has property name" ;
  rdfs:range loin:PropertyName ;
.
loin:hasProvider
  rdf:type owl:ObjectProperty ;
  rdfs:domain loin:InformationDeliveryMilestone ;
  rdfs:label "has provider" ;
  rdfs:range loin:InformationProvider ;
.
loin:hasPurpose
  rdf:type owl:ObjectProperty ;
  rdfs:domain loin:InformationDeliveryMilestone ;
  rdfs:label "has purpose" ;
  rdfs:range loin:Purpose ;
.
loin:hasReceiver
  rdf:type owl:ObjectProperty ;
  rdfs:domain loin:InformationDeliveryMilestone ;
  rdfs:label "has information receiver" ;
  rdfs:range loin:InformationReceiver ;
.
loin:hasReferenceSource
  rdf:type owl:ObjectProperty ;
  rdfs:domain [
      rdf:type owl:Class ;
      owl:unionOf (
          loin:BreakdownStructure
          loin:OntologyDataDefinition
        ) ;
    ] ;
  rdfs:label "has reference source" ;
  rdfs:range xsd:anyURI ;
  rdfs:range owl:Thing ;
.
loin:hasRequirement
  rdf:type owl:ObjectProperty ;
  rdfs:domain loin:IDSDataDefinition ;
  rdfs:label "has requirement" ;
  rdfs:range loin:IDSFacetDefinition ;
.
loin:hasRequirementType
  rdf:type owl:ObjectProperty ;
  rdfs:domain loin:IDSFacetDefinition ;
  rdfs:label "has requirement type" ;
  rdfs:range loin:IDSRequirementType ;
.
loin:hasRestrictionType
  rdf:type owl:ObjectProperty ;
  rdfs:domain loin:IDSFacetParameter ;
  rdfs:label "has restriction type" ;
  rdfs:range loin:IDSRestrictionType ;
.
loin:hasValue
  rdf:type owl:ObjectProperty ;
  rdfs:domain loin:Attribute ;
  rdfs:domain loin:Material ;
  rdfs:domain loin:Property ;
  rdfs:label "has value" ;
  rdfs:range loin:Value ;
.
loin:isRelatedToContainerDescription
  rdf:type owl:ObjectProperty ;
  rdfs:domain loin:InformationDeliveryMilestone ;
  rdfs:domain loin:Purpose ;
  rdfs:label "is related to container description" ;
  rdfs:label "isRelatedToContainerDescription" ;
  rdfs:range Container:ContainerDescription ;
.
loin:isRelatedToContainerDocument
  rdf:type owl:ObjectProperty ;
  rdf:type owl:SymmetricProperty ;
  rdfs:domain loin:Document ;
  rdfs:label "is related to container document" ;
  rdfs:range Container:Document ;
.
loin:isRelatedToContainerLinkset
  rdf:type owl:ObjectProperty ;
  rdfs:domain loin:Document ;
  rdfs:label "is related to container linkset" ;
  rdfs:range Container:Linkset ;
.
loin:isRelatedToContainerParty
  rdf:type rdf:Property ;
  rdfs:domain loin:Actor ;
  rdfs:label "is related to container party" ;
  rdfs:range Container:Party ;
.
loin:isRelatedToLinksetIdentifier
  rdf:type rdf:Property ;
  rdfs:domain loin:IdentifierType ;
  rdfs:label "is related to linkset identifier" ;
  rdfs:range Linkset:Identifier ;
.
loin:isRelatedToLoinDocument
  rdf:type owl:ObjectProperty ;
  rdfs:domain loin:InformationContent ;
  rdfs:label "is related to Loin document" ;
  rdfs:range loin:Document ;
.
loin:name
  rdf:type owl:AnnotationProperty ;
  rdfs:range xsd:string ;
.
loin:one-dimensional
  rdf:type loin:Dimensionality ;
.
loin:parametric
  rdf:type loin:ParametricBehaviour ;
.
loin:preliminaryDesign
  rdf:type loin:InformationDeliveryMilestone ;
  rdfs:comment "Example from ISO 17412-1:2022 - Annex B" ;
  rdfs:label "Preliminary design" ;
.
loin:real-world
  rdf:type loin:Appearance ;
.
loin:realistic
  rdf:type loin:Appearance ;
.
loin:relative
  rdf:type loin:Location ;
.
loin:requested
  rdf:type owl:DatatypeProperty ;
  rdfs:domain loin:Geometry ;
  rdfs:domain loin:GeometrySpecification ;
  rdfs:domain loin:Information ;
  rdfs:range xsd:boolean ;
.
loin:simplified
  rdf:type loin:Detail ;
.
loin:specifiedByIdentifier
  rdf:type rdf:Property ;
  rdfs:domain loin:InformationContent ;
  rdfs:label "specified by identifier" ;
  rdfs:range loin:Identifier ;
.
loin:structuralAnalysis
  rdf:type loin:Purpose ;
  loin:description "Structural analysis - example from ISO 17412-1:2022 - Annex B" ;
  rdfs:comment "Example from ISO 17412-1:2022 - Annex B" ;
  rdfs:label "Structural analysis" ;
.
loin:symbolic
  rdf:type loin:Appearance ;
.
loin:three-dimensional
  rdf:type loin:Dimensionality ;
.
loin:two-dimensional
  rdf:type loin:Dimensionality ;
.
loin:value
  rdf:type owl:DatatypeProperty ;
.
loin:visualization
  rdf:type loin:Purpose ;
  loin:description "Visualization - example from ISO 17412-1:2022 - Annex B" ;
  rdfs:comment "Example from ISO 17412-1:2022 - Annex B" ;
  rdfs:label "Visualization" ;
.
loin:zero-dimensional
  rdf:type loin:Dimensionality ;
.
